coq/theories/clc_arity_spine.v
@@ -1,3 +1,5 @@
+(* The file presents various lemmas for manipulating arities and spine forms. *)
+
 From mathcomp Require Import ssreflect ssrbool eqtype ssrnat seq.
 From Coq Require Import ssrfun Utf8 Classical.
 Require Import AutosubstSsr ARS
